full proof in stlc0.v
There are two full no-admit proofs now, one for soundness
one for termination on a language with termination capabilities.
Next step: integrate.

dev2019/stlc0.v
@@ -7,6 +7,8 @@
 (* Starting point: https://github.com/TiarkRompf/minidot/blob/master/dev2015/nano2.v *)
 (* Starting point: https://github.com/TiarkRompf/scala-escape/blob/master/coq/stlc1.v *)
 
+(* The goal of this version is to be as simple as possible. 
+   No subtyping, env not part of val_type relation. *)
 
 Require Export Arith.EqNat.
 Require Export Arith.Le.
@@ -307,30 +309,25 @@ Qed.
 Inductive wf_env : venv -> tenv -> Prop := 
 | wfe_nil : forall n, wf_env (Def vl nil nil n) (Def ty nil nil n)
 | wfe_cons : forall v t vs ts n,
-    val_type (expand_env vs v n) v t ->
+    val_type v t ->
     wf_env vs ts ->
     get_inv_idx vs = get_inv_idx ts ->
     wf_env (expand_env vs v n) (expand_env ts t n)
 
-with val_type : venv -> vl -> ty -> Prop := 
-| v_bool: forall venv b,
-    val_type venv (vbool b) TBool
-| v_abs: forall env venv tenv y T1 T2 m, (* NEW: TRec wrapper *)
+with val_type : vl -> ty -> Prop := 
+| v_bool: forall b,
+    val_type (vbool b) TBool
+| v_abs: forall venv tenv y T1 T2 m, (* NEW: TRec wrapper *)
     wf_env venv tenv ->
     has_type (expand_env (expand_env tenv (TRec (TFun T1 m T2)) Second) T1 m) y First T2 ->
-    val_type env (vabs venv m y) (TFun T1 m T2)
-| v_rec: forall env v T,  (* NEW *)
-    val_type env v T ->
-    val_type env (vrec v) (TRec T)
-| v_cap: forall env,
-    val_type env vcap TCap (* NEW *)
+    val_type (vabs venv m y) (TFun T1 m T2)
+| v_rec: forall v T,  (* NEW *)
+    val_type v T ->
+    val_type (vrec v) (TRec T)
+| v_cap:
+    val_type vcap TCap (* NEW *)
 .
 
-
-(* type equivalence: only via reflexivity *)
-Inductive stp: venv -> ty -> venv -> ty -> Prop :=
-| stp_refl: forall G1 G2 T,
-   stp G1 T G2 T.
 
 Hint Constructors val_type.
 Hint Constructors wf_env.
@@ -391,11 +388,6 @@ Qed.
 Hint Immediate wf_idx.
 
 
-Lemma valtp_extend : forall vs v v1 T n,
-                       val_type vs v T ->
-                       val_type (expand_env vs v1 n) v T.
-Proof. intros. induction H; eauto. Qed.
-
 Lemma index_extend : forall X vs n a (T: X),
                        index n vs = Some T ->
                        index n (a::vs) = Some T.
@@ -424,21 +416,11 @@ Proof.
     inversion H; simpl; try rewrite E; auto.
 Qed.
 
-(*
-Lemma index_safe_ex: forall Hl1 Hl2 Gl1 Gl2 Hidx Gidx TF i,
-   wf_env (Def vl Hl1 Hl2 Hidx) (Def ty Gl1 Gl2 Gidx) ->
-   index i Gl1 = Some TF ->
-   exists v, index i Hl1 = Some v.
-Proof. intros.
-  apply wf_length in H. destruct H as [L _]. simpl in L.
-  
-Qed.
-*)
 
 Lemma lookup_safe_ex: forall H1 G1 TF x,
              wf_env H1 G1 ->
              lookup x G1 = Some TF ->
-             exists v, lookup x H1 = Some v /\ val_type H1 v TF.
+             exists v, lookup x H1 = Some v /\ val_type v TF.
 Proof. intros. induction H.
   - (* Case "nil". *) inversion H0. destruct x; destruct c; destruct (ble_nat n i); inversion H1.
   - (* Case "cons". *) destruct vs as [vl1 vl2 vidx]. destruct ts as [tl1 tl2 tidx].
@@ -455,21 +437,21 @@ Proof. intros. induction H.
         { (* SSSCase "miss". *)
           intros E.
           assert (beq_nat i (length vl1) = false). eauto.
-          assert (exists v0, lookup (V First i) (Def vl vl1 vl2 vidx) = Some v0 /\ val_type (Def vl vl1 vl2 vidx) v0 TF) as HI.
+          assert (exists v0, lookup (V First i) (Def vl vl1 vl2 vidx) = Some v0 /\ val_type v0 TF) as HI.
           eapply IHwf_env. simpl. rewrite E in H0. eauto.
           inversion HI as [v0 HI1]. inversion HI1.
-          eexists. econstructor. eapply lookup_extend; eauto. eapply valtp_extend; eauto. }
+          eexists. econstructor. eapply lookup_extend; eauto. eauto. }
      * (* SSCase "Second". *)
-       assert (exists v0, lookup (V First i) (Def vl vl1 vl2 vidx) = Some v0 /\ val_type (Def vl vl1 vl2 vidx) v0 TF) as HI.
+       assert (exists v0, lookup (V First i) (Def vl vl1 vl2 vidx) = Some v0 /\ val_type v0 TF) as HI.
        eapply IHwf_env. simpl. eauto.
        inversion HI as [v0 HI1]. inversion HI1.
-       eexists. econstructor. eapply lookup_extend; eauto. eapply valtp_extend; eauto.
+       eexists. econstructor. eapply lookup_extend; eauto. eauto.
    + (* SCase "VSnd". *) destruct n; simpl in H0; simpl in H2.
      * (* SSCase "First". *)
-       assert (exists v0, lookup (V Second i) (Def vl vl1 vl2 vidx) = Some v0 /\ val_type (Def vl vl1 vl2 vidx) v0 TF) as HI.
+       assert (exists v0, lookup (V Second i) (Def vl vl1 vl2 vidx) = Some v0 /\ val_type v0 TF) as HI.
        eapply IHwf_env. simpl. eauto.
        inversion HI as [v0 HI1]. inversion HI1.
-       eexists. econstructor. eapply lookup_extend; eauto. eapply valtp_extend; eauto.
+       eexists. econstructor. eapply lookup_extend; eauto. eauto.
      * (* SSCase "Second". *)
        case_eq (beq_nat i (length tl2)).
         { (* SSSCase "hit". *)
@@ -481,41 +463,27 @@ Proof. intros. induction H.
         { (* SSSCase "miss". *)
           intro E.
           assert (beq_nat i (length vl2) = false). eauto.
-          assert (exists v0, lookup (V Second i) (Def vl vl1 vl2 vidx) = Some v0 /\ val_type (Def vl vl1 vl2 vidx) v0 TF) as HI.
+          assert (exists v0, lookup (V Second i) (Def vl vl1 vl2 vidx) = Some v0 /\ val_type v0 TF) as HI.
           eapply IHwf_env. simpl. destruct (ble_nat tidx i). inversion H0. rewrite E in H0. rewrite H0. rewrite E. auto. auto.
           inversion HI as [v0 HI1]. inversion HI1.
-          eexists. econstructor. eapply lookup_extend; eauto. eapply valtp_extend; eauto. }
+          eexists. econstructor. eapply lookup_extend; eauto. eauto. }
 Qed.
   
-Inductive res_type: venv -> option vl -> ty -> Prop :=
-| not_stuck: forall venv v T,
-      val_type venv v T ->
-      res_type venv (Some v) T.
+Inductive res_type: option vl -> ty -> Prop :=
+| not_stuck: forall v T,
+      val_type v T ->
+      res_type (Some v) T.
 
 Hint Constructors res_type.
 Hint Resolve not_stuck.
 
 
-Lemma valtp_widen: forall vf H1 H2 T1 T2,
-  val_type H1 vf T1 ->
-  stp H1 T1 H2 T2 ->
-  val_type H2 vf T2.
-Proof.
-  intros. generalize dependent T2. induction H; intros.
-  - inversion H0. eauto.
-  - inversion H1. eauto.
-  - inversion H0. eapply v_rec. eapply IHval_type. eapply stp_refl.
-  - inversion H0. eauto. 
-Qed.
-
-Lemma invert_abs: forall venv vf vx T1 n T2,
-  val_type venv vf (TFun T1 n T2) ->
+Lemma invert_abs: forall vf T1 n T2,
+  val_type vf (TFun T1 n T2) ->
   exists env tenv y T3 T4,
     vf = (vabs env n y) /\
     wf_env env tenv /\
-    has_type (expand_env (expand_env tenv (TRec (TFun T3 n T4)) Second) T3 n) y First T4 /\
-    stp venv T1 (expand_env (expand_env env (vrec vf) Second) vx n) T3 /\
-    stp (expand_env (expand_env env (vrec vf) Second) vx n) T4 venv T2.
+    has_type (expand_env (expand_env tenv (TRec (TFun T3 n T4)) Second) T3 n) y First T4.
 Proof.
   intros. inversion H. repeat eexists; repeat eauto.
 Qed.
@@ -527,20 +495,6 @@ Proof.
   intros. destruct venv0. destruct c; simpl; eauto. 
 Qed.
 
-Lemma val_type_sanitize_any : forall n venv res T,
-  val_type venv res T ->
-  val_type (sanitize_any venv n) res T.
-Proof.
-  intros. induction H; eauto. 
-Qed.
-
-Lemma val_type_sanitize : forall env res T n,
-  val_type (sanitize_env n env) res T ->
-  val_type env res T.
-Proof.
-  intros. induction H; eauto.
-Qed.
-
 Lemma wf_sanitize_any : forall n venv tenv,
    wf_env venv tenv ->
    wf_env (sanitize_any venv n) (sanitize_any tenv n).
@@ -549,8 +503,7 @@ Proof.
   - simpl. eapply wfe_nil.
   - eapply wfe_cons in IHwf_env.
     rewrite <-ext_sanitize_commute. rewrite <-ext_sanitize_commute.
-    eauto. eauto. rewrite ext_sanitize_commute.
-    eapply val_type_sanitize_any in H. eauto. eauto.
+    eauto. eauto. eauto. 
 Qed.  
 
 Lemma wf_sanitize : forall n venv tenv,
@@ -573,7 +526,7 @@ Hint Immediate wf_sanitize.
 
 Theorem full_safety : forall k e n tenv venv res T,
   teval k venv e n = Some res -> has_type tenv e n T -> wf_env venv tenv ->
-  res_type venv res T.
+  res_type res T.
 
 Proof.
   intros k. induction k.
@@ -587,44 +540,24 @@ Proof.
     subst.
     destruct (lookup_safe_ex (sanitize_env n venv0) (sanitize_env n tenv0) T v) as [va [I V]]; eauto. 
 
-    rewrite I. eapply not_stuck. eapply val_type_sanitize. eapply V.
+    rewrite I. eapply not_stuck. eapply V. 
 
   - (* Case "App". *)
-    remember (teval k venv0 e1 Second) as tf.
-    subst T. subst n0.
-    
+    subst T. subst. remember (teval k venv0 e1 Second) as tf.
     destruct tf as [rf|]; try inversion H3. 
-    assert (res_type venv0 rf (TFun T1 m T2)) as HRF. (* SCase "HRF". *) subst. eapply IHk; eauto.
-    inversion HRF as [? vf].
+    assert (res_type rf (TFun T1 m T2)) as HRF. { eapply IHk; eauto. }
+    inversion HRF as [vf TF HVF]. inversion HVF.
+    subst rf. subst vf. 
 
-    subst rf. remember vf as rvf. destruct vf; subst rvf; inversion H7. (* try (subst rvf; solve inversion). *)
-    assert (c = m). destruct m; destruct c; try inversion H18; eauto. (* try (subst rvf; solve inversion); eauto.*) subst c. (* subst rvf. *)
     remember (teval k venv0 e2 m0) as tx.
-
     destruct tx as [rx|]; try inversion H3.
-    assert (res_type venv0 rx T1) as HRX. (* SCase "HRX". *) subst. eapply IHk; eauto.
-    inversion HRX as [? vx]. 
+    assert (res_type rx T1) as HRX. { subst. eapply IHk; eauto. }
+    inversion HRX as [vx]. subst rx T.
 
-    destruct (invert_abs venv0 (vabs e m t) vx T1 m T2) as
-        [env1' [tenv1' [y0 [T3' [T4' [EF [WF [HTY [STX STY]]]]]]]]]. eauto.
-    (* now we know it's a closure, and we have has_type evidence *)
+    subst. eapply IHk. eauto. eauto.
+    (* WF on expanded env *)
+    constructor. eauto. constructor. eauto. eauto. eauto. apply wf_idx. eauto. 
 
-    inversion EF. subst e. subst y0. clear EF.
-    subst rx.
-
-    assert (res_type (expand_env (expand_env env1' (vrec (vabs venv2 m t)) Second) vx m) res T4') as HRY.
-        (* SSSCase "HRY". *)
-          subst. eapply IHk; eauto.
-        (* wf_env f x *) econstructor. eapply valtp_widen; eauto.
-        (* wf_env f   *) econstructor. eapply v_rec. eapply v_abs; eauto.
-          eauto.
-          apply wf_idx. assumption.
-          apply wf_idx. econstructor. eauto. assumption. apply wf_idx. assumption.
-
-    inversion HRY as [? vy].
-
-    eapply not_stuck. eapply valtp_widen; eauto.
-    
   - (* Case "Abs". *) intros. inversion H. inversion H0.
     eapply not_stuck. eapply v_abs; eauto.
     eauto.
@@ -632,7 +565,7 @@ Proof.
     remember (teval k venv0 e1 n) as tevr.
 
     destruct tevr as [revr|]; try inversion H3.
-    assert (res_type venv0 revr (TRec T)) as HRR. {
+    assert (res_type revr (TRec T)) as HRR. {
      subst. eapply IHk; eauto.
     }
 
@@ -640,7 +573,7 @@ Proof.
 
     remember (teval k venv0 e2 n) as tevc. 
     destruct tevc as [revc|]; try inversion H11.
-    assert (res_type venv0 revc TCap) as HRC. {
+    assert (res_type revc TCap) as HRC. {
       subst. eapply IHk; eauto.
     }
     inversion HRC as [? vc]. inversion H2. subst.
@@ -665,11 +598,11 @@ Definition tevaln env e cl v := exists nm, forall n, n > nm -> teval n env e cl 
 
 
 (* need to use Fixpoint because of positivity restriction *)
-Fixpoint val_type_tnt (env:venv) (v:vl) (T:ty): Prop := match v, T with
+Fixpoint val_type_tnt (v:vl) (T:ty): Prop := match v, T with
 | vbool b, TBool => True
 | vabs env clv y, TFun T1 clt T2 => (clv = clt) /\
-  (forall vx, val_type_tnt env vx T1 ->
-     exists v, tevaln (expand_env (expand_env env (vrec (vabs env clv y)) Second) vx clv) y First v /\ val_type_tnt env v T2)
+  (forall vx, val_type_tnt vx T1 ->
+     exists v, tevaln (expand_env (expand_env env (vrec (vabs env clv y)) Second) vx clv) y First v /\ val_type_tnt v T2)
 | vrec v, TRec T => True (* NEW: rec, but we can't do anything with it *)
 | _,_ => False
 end.
@@ -678,8 +611,7 @@ end.
 Inductive wf_env_tnt : venv -> tenv -> Prop := 
 | wfe_tnt_nil : forall n, wf_env_tnt (Def vl nil nil n) (Def ty nil nil n)
 | wfe_tnt_env : forall v t vs ts n,
-    val_type_tnt (expand_env vs v n) v t ->
-    (* val_type (expand_env vs v n) v t ?? *) (* vrec v ?? *)
+    val_type_tnt v t ->
     wf_env_tnt vs ts ->
     get_inv_idx vs = get_inv_idx ts ->
     wf_env_tnt (expand_env vs v n) (expand_env ts t n)
@@ -722,35 +654,12 @@ Qed.
 
 Hint Immediate wf_length_tnt.
 
-Lemma valtp_extend_tnt : forall vs v v1 T n,
-                       val_type_tnt vs v T ->
-                       val_type_tnt (expand_env vs v1 n) v T.
-Proof.
-  intros. induction v.
-  - (* bool *) admit.
-  - (* abs *) admit.
-  - (* rec *) admit.
-  - (* cap *) admit.
-Admitted.
-
-(* NOTE: will needed (closed T vs) ! *)
-Lemma valtp_shrink_tnt : forall vs v v1 T n,
-                       val_type_tnt (expand_env vs v1 n) v T ->
-                       val_type_tnt vs v T.
-Proof.
-  intros. induction v.
-  - (* bool *) admit.
-  - (* abs *) admit.
-  - (* rec *) admit.
-  - (* cap *) admit.
-Admitted.
-
 
 
 Lemma lookup_safe_ex_tnt: forall H1 G1 TF x,
              wf_env_tnt H1 G1 ->
              lookup x G1 = Some TF ->
-             exists v, lookup x H1 = Some v /\ val_type_tnt H1 v TF.
+             exists v, lookup x H1 = Some v /\ val_type_tnt v TF.
 Proof. intros. induction H.
   - (* Case "nil". *) inversion H0. destruct x; destruct c; destruct (ble_nat n i); inversion H1.
   - (* Case "cons". *) destruct vs as [vl1 vl2 vidx]. destruct ts as [tl1 tl2 tidx].
@@ -767,21 +676,21 @@ Proof. intros. induction H.
         { (* SSSCase "miss". *)
           intros E.
           assert (beq_nat i (length vl1) = false). eauto.
-          assert (exists v0, lookup (V First i) (Def vl vl1 vl2 vidx) = Some v0 /\ val_type_tnt (Def vl vl1 vl2 vidx) v0 TF) as HI.
+          assert (exists v0, lookup (V First i) (Def vl vl1 vl2 vidx) = Some v0 /\ val_type_tnt  v0 TF) as HI.
           eapply IHwf_env_tnt. simpl. rewrite E in H0. eauto.
           inversion HI as [v0 HI1]. inversion HI1.
-          eexists. econstructor. eapply lookup_extend; eauto. eapply valtp_extend_tnt; eauto. }
+          eexists. econstructor. eapply lookup_extend; eauto. eauto. }
      * (* SSCase "Second". *)
-       assert (exists v0, lookup (V First i) (Def vl vl1 vl2 vidx) = Some v0 /\ val_type_tnt (Def vl vl1 vl2 vidx) v0 TF) as HI.
+       assert (exists v0, lookup (V First i) (Def vl vl1 vl2 vidx) = Some v0 /\ val_type_tnt v0 TF) as HI.
        eapply IHwf_env_tnt. simpl. eauto.
        inversion HI as [v0 HI1]. inversion HI1.
-       eexists. econstructor. eapply lookup_extend; eauto. eapply valtp_extend_tnt; eauto.
+       eexists. econstructor. eapply lookup_extend; eauto. eauto. 
    + (* SCase "VSnd". *) destruct n; simpl in H0; simpl in H2.
      * (* SSCase "First". *)
-       assert (exists v0, lookup (V Second i) (Def vl vl1 vl2 vidx) = Some v0 /\ val_type_tnt (Def vl vl1 vl2 vidx) v0 TF) as HI.
+       assert (exists v0, lookup (V Second i) (Def vl vl1 vl2 vidx) = Some v0 /\ val_type_tnt v0 TF) as HI.
        eapply IHwf_env_tnt. simpl. eauto.
        inversion HI as [v0 HI1]. inversion HI1.
-       eexists. econstructor. eapply lookup_extend; eauto. eapply valtp_extend_tnt; eauto.
+       eexists. econstructor. eapply lookup_extend; eauto. eauto.
      * (* SSCase "Second". *)
        case_eq (beq_nat i (length tl2)).
         { (* SSSCase "hit". *)
@@ -793,42 +702,12 @@ Proof. intros. induction H.
         { (* SSSCase "miss". *)
           intro E.
           assert (beq_nat i (length vl2) = false). eauto.
-          assert (exists v0, lookup (V Second i) (Def vl vl1 vl2 vidx) = Some v0 /\ val_type_tnt (Def vl vl1 vl2 vidx) v0 TF) as HI.
+          assert (exists v0, lookup (V Second i) (Def vl vl1 vl2 vidx) = Some v0 /\ val_type_tnt v0 TF) as HI.
           eapply IHwf_env_tnt. simpl. destruct (ble_nat tidx i). inversion H0. rewrite E in H0. rewrite H0. rewrite E. auto. auto.
           inversion HI as [v0 HI1]. inversion HI1.
-          eexists. econstructor. eapply lookup_extend; eauto. eapply valtp_extend_tnt; eauto. }
+          eexists. econstructor. eapply lookup_extend; eauto. eauto. }
 Qed.
 
-
-
-  
-Lemma invert_abs_tnt: forall venv vf T1 cl T2,
-  val_type_tnt venv vf (TFun T1 cl T2) ->
-  exists env y,
-    vf = (vabs env cl y) /\ 
-    (forall vx, val_type_tnt venv vx T1 ->
-       exists v, tevaln (expand_env (expand_env env (vrec vf) Second) vx cl) y First v /\ val_type_tnt venv v T2).
-Proof.
-  intros. simpl in H. destruct vf.
-  - inversion H.
-  - destruct H. subst c. exists e. exists t. split. eauto. admit. (* wrong env, need widen *)
-  - inversion H.
-  - inversion H. 
-Admitted.
-
-Lemma val_type_sanitize_any_tnt : forall n venv res T,
-  val_type_tnt venv res T ->
-  val_type_tnt (sanitize_any venv n) res T.
-Proof.
-  intros. admit. (* induction H; eauto. *)
-Admitted.
-
-Lemma val_type_sanitize_tnt : forall env res T n,
-  val_type_tnt (sanitize_env n env) res T ->
-  val_type_tnt env res T.
-Proof.
-  intros. admit. (* induction H; eauto. *)
-Admitted.
 
 Lemma wf_idx_tnt : forall vs ts,
       wf_env_tnt vs ts ->
@@ -848,8 +727,7 @@ Proof.
   - simpl. eapply wfe_tnt_nil.
   - eapply wfe_tnt_env in IHwf_env_tnt.
     rewrite <-ext_sanitize_commute. rewrite <-ext_sanitize_commute.
-    eauto. eauto. rewrite ext_sanitize_commute.
-    eapply val_type_sanitize_any_tnt in H. eauto. eauto.
+    eauto. eauto. eauto. 
 Qed.  
 
 Lemma wf_sanitize_tnt : forall n venv tenv,
@@ -871,7 +749,7 @@ Hint Immediate wf_sanitize_tnt.
 
 Theorem full_total_safety : forall e cl tenv T,
   has_type tenv e cl T -> forall venv, wf_env_tnt venv tenv ->
-  exists v, tevaln venv e cl v /\ val_type_tnt venv v T.
+  exists v, tevaln venv e cl v /\ val_type_tnt v T.
 
 Proof.
   intros ? ? ? ? W.
@@ -886,14 +764,14 @@ Proof.
     destruct (lookup_safe_ex_tnt (sanitize_env n venv0) (sanitize_env n env0) T1 x) as [v IV]. eauto. eauto. 
     inversion IV as [I V]. 
 
-    exists v. split. exists 0. intros. destruct n0. omega. simpl. rewrite I. eauto. eapply val_type_sanitize_tnt. eapply V.
+    exists v. split. exists 0. intros. destruct n0. omega. simpl. rewrite I. eauto. eapply V.
 
   - (* Case "App". *)
     destruct (IHW1 venv0 WFE) as [vf [IW1 HVF]].
     destruct (IHW2 venv0 WFE) as [vx [IW2 HVX]].
-    
-    eapply invert_abs_tnt in HVF.
-    destruct HVF as [venv1 [y [HF IHF]]].
+
+    simpl in HVF. destruct vf; try contradiction.    
+    destruct HVF  as [? IHF].
 
     destruct (IHF vx HVX) as [vy [IW3 HVY]].
 
@@ -902,32 +780,21 @@ Proof.
       destruct IW1 as [nf IWF].
       destruct IW2 as [nx IWX].
       destruct IW3 as [ny IWY].
-      exists (S (nf+nx+ny)). intros. destruct n0. omega. simpl.
-      rewrite IWF. subst vf. rewrite IWX. rewrite IWY. eauto.
+      exists (S (nf+nx+ny)). intros. destruct n0. omega. simpl. subst c.
+      rewrite IWF. rewrite IWX. rewrite IWY. eauto.
       omega. omega. omega.
     }
     eapply HVY.
     
   - (* Case "Abs". *)
     eexists. split. exists 0. intros. destruct n0. omega. simpl. eauto.
-    simpl. repeat split; eauto.  intros. 
-(*    assert (stpd2 true venv0 T1 (vx::venv0) T1). eapply stpd2_extend2. eapply stpd2_refl; eauto. eu.
-    assert (stpd2 true (vx::venv0) T2 venv0 T2). eapply stpd2_extend1. eapply stpd2_refl; eauto. eu. *)
+    simpl. repeat split; eauto. intros. 
 
-    remember (expand_env
-         (expand_env (sanitize_env n venv0)
-            (vrec
-               (vabs (sanitize_env n venv0) m y))
-            Second) vx m) as venv1.
-
-    remember (expand_env
-             (expand_env (sanitize_env n env0)
-                (TRec (TFun T1 m T2)) Second) T1
-             m) as tenv1.
+    eapply IHW.
+    constructor. eauto. constructor. simpl; eauto. eauto.
+    eapply wf_idx_tnt. eauto. eapply wf_idx_tnt.
+    constructor. simpl; eauto. eauto. eapply wf_idx_tnt. eauto. 
     
-    assert (val_type_tnt venv1 vx T1). { subst. eapply valtp_extend_tnt. eapply valtp_extend_tnt. eauto. }
-    assert (wf_env_tnt venv1 tenv1). { subst. eapply wfe_tnt_env. eauto. eapply wfe_tnt_env. simpl. auto. eauto. eapply wf_idx_tnt. eapply wf_sanitize_tnt. eauto. eapply wf_idx_tnt. eapply wfe_tnt_env. simpl. auto. eauto. eapply wf_idx_tnt. eapply wf_sanitize_tnt. eauto. }
-    specialize (IHW venv1 H1). destruct IHW as [v [? ?]]. exists v. split. eauto. eapply valtp_shrink_tnt. eapply valtp_shrink_tnt. subst. eauto. 
   - (* Case tunrec *)
     destruct (IHW2 _ WFE) as [v [HEV HVL]].
     simpl in HVL. destruct v; inversion HVL.
